src/Examples/ReplicatedDisk/ReplicatedDiskImpl.v
@@ -1,0 +1,1082 @@
+Require Import POCS.
+
+Require Import TwoDiskAPI.
+Require Import OneDiskAPI.
+
+(**
+ReplicatedDisk provides a single-disk API on top of two disks, handling disk
+failures with replication.
+*)
+
+
+Module ReplicatedDisk (td : TwoDiskAPI).  (* <: OneDiskAPI. *)
+
+  Import ProcNotations EqualDecNotation.
+  Open Scope proc_scope.
+
+  (* FIXME: this should be in tactical but was deleted by accident *)
+  Ltac destruct_tuple :=
+    match goal with
+    | [ H: context[let '(a, b) := ?p in _] |- _ ] =>
+      let a := fresh a in
+      let b := fresh b in
+      destruct p as [a b]
+    | [ |- context[let '(a, b) := ?p in _] ] =>
+      let a := fresh a in
+      let b := fresh b in
+      destruct p as [a b]
+    end.
+
+  Definition read (a:addr) : proc Op block :=
+    mv0 <- td.read d0 a;
+    match mv0 with
+    | Working v => Ret v
+    | Failed =>
+      mv2 <- td.read d1 a;
+      match mv2 with
+      | Working v => Ret v
+      | Failed => Ret block0
+      end
+    end.
+
+  Definition write (a:addr) (b:block) : proc Op unit :=
+    _ <- td.write d0 a b;
+    _ <- td.write d1 a b;
+    Ret tt.
+
+  Definition size : proc Op nat :=
+    msz <- td.size d0;
+    match msz with
+    | Working sz => Ret sz
+    | Failed =>
+      msz <- td.size d1;
+      match msz with
+      | Working sz => Ret sz
+      | Failed => Ret 0
+      end
+    end.
+
+  (*
+  (** [sizeInit] computes the size during initialization; it may return None if
+  the sizes of the underlying disks differ. *)
+  Definition sizeInit : proc Op (option nat) :=
+    sz1 <- td.size d0;
+    sz2 <- td.size d1;
+    match sz1 with
+    | Working sz1 =>
+      match sz2 with
+      | Working sz2 =>
+        if sz1 == sz2 then Ret (Some sz1) else Ret None
+      | Failed => Ret (Some sz1)
+      end
+    | Failed =>
+      match sz2 with
+      | Working sz2 => Ret (Some sz2)
+      | Failed => Ret None
+      end
+    end.
+
+  (* Recursively initialize block a and below. For simplicity, we make the disks
+  match by setting every block to [block0]. *)
+  Fixpoint init_at (a:nat) : proc Op unit :=
+    match a with
+    | 0 => Ret tt
+    | S a =>
+      _ <- td.write d0 a block0;
+      _ <- td.write d1 a block0;
+      init_at a
+    end.
+
+  (* Initialize every disk block *)
+  Definition init' : proc Op InitResult :=
+    size <- sizeInit;
+    match size with
+    | Some sz =>
+      _ <- init_at sz;
+      Ret Initialized
+    | None =>
+      Ret InitFailed
+    end.
+  *)
+
+  (*
+  Definition init := then_init td.init init'.
+   *)
+
+
+  (**
+   * Helper theorems and tactics for proofs.
+   *)
+
+  Theorem exists_tuple2 : forall A B (P: A * B -> Prop),
+      (exists a b, P (a, b)) ->
+      (exists p, P p).
+  Proof.
+    intros.
+    repeat deex; eauto.
+  Qed.
+
+  Tactic Notation "eexist_tuple" ident(a) ident(b) :=
+    match goal with
+    | [ |- exists (_:?aT * ?bT), _ ] =>
+      let a := fresh a in
+      let b := fresh b in
+      evar (a : aT);
+      evar (b : bT);
+      exists (a, b);
+      subst a;
+      subst b
+    end.
+
+  Ltac simplify :=
+    repeat match goal with
+           | |- forall _, _ => intros
+           | _ => deex
+           | _ => destruct_tuple
+           | [ u: unit |- _ ] => destruct u
+           | |- _ /\ _ => split; [ solve [auto] | ]
+           | |- _ /\ _ => split; [ | solve [auto] ]
+           | |- exists (_: disk*(disk -> Prop)), _ => eexist_tuple d F
+           | |- exists (_: disk*disk), _ => eexist_tuple d_0 d_1
+           | |- exists (_: disk*_), _ => apply exists_tuple2
+           | _ => progress simpl in *
+           | _ => progress safe_intuition
+           | _ => progress subst
+           | _ => progress autorewrite with upd in *
+           end.
+
+  (* The [finish] tactic tries a number of techniques to solve the goal. *)
+  Ltac finish :=
+    repeat match goal with
+           | _ => solve_false
+           | _ => congruence
+           | _ => solve [ intuition (subst; eauto; try congruence) ]
+           | _ =>
+             (* if we can solve all the side conditions automatically, then it's
+             safe to run descend and create existential variables *)
+             descend; (intuition eauto);
+             lazymatch goal with
+             | |- proc_ok _ _ _ _ => idtac
+             | _ => fail
+             end
+           end.
+  
+  Ltac monad_simpl :=
+    repeat match goal with
+           | |- proc_ok _ (Bind (Ret _) _) _ _ =>
+             eapply proc_ok_expand; [ apply monad_left_id | ]
+           | |- proc_ok _ (Bind (Bind _ _) _) _ _ =>
+             eapply proc_ok_expand; [ apply monad_assoc | ]
+           end.
+  
+  Ltac step_proc :=
+    intros;
+    match goal with
+    | |- proc_ok _ (Ret _) _ _ =>
+      eapply ret_spec
+    | |- proc_ok _ _ _ _ =>
+      monad_simpl;
+      eapply proc_ok_rx; [ solve [ eauto ] | ]
+    | [ H: proc_ok _ ?p _ _
+        |- proc_ok _ ?p _ _ ] =>
+      eapply spec_impl_relations; [ unfold spec_impl | eapply H ]
+    end;
+    intros; simpl;
+    cbn [pre post recovered] in *;
+    repeat match goal with
+           | [ H: _ /\ _ |- _ ] => destruct H
+           | [ |- rec_noop _ _ _ ] => eauto
+           | [ |- forall _, _ ] => intros
+           | [ |- exists (_:unit), _ ] => exists tt
+           | [ |- _ /\ _ ] => split; [ solve [ trivial ] | ]
+           | [ |- _ /\ _ ] => split; [ | solve [ trivial ] ]
+           | _ => solve [ trivial ]
+           | _ => progress subst
+           | _ => progress autounfold in *
+           end.
+
+  Ltac step :=
+    step_proc; simplify; finish.
+
+  (**
+   * Specifications and proofs about our implementation of the replicated disk API,
+   * without considering our recovery.
+   *
+   * These intermediate specifications separate reasoning about the
+   * implementations from recovery behavior.
+   *)
+
+  Theorem both_disks_not_missing : forall (state: TwoDiskBaseAPI.State),
+      disk0 state ?|= missing ->
+      disk1 state ?|= missing ->
+      False.
+  Proof.
+    destruct state; unfold missing; simpl; intuition auto.
+  Qed.
+
+  Hint Resolve both_disks_not_missing : false.
+
+  Theorem missing0_implies_any : forall (state: TwoDiskBaseAPI.State) P,
+      disk0 state ?|= missing ->
+      disk0 state ?|= P.
+  Proof.
+    destruct state; unfold missing; simpl; intuition auto.
+  Qed.
+
+  Theorem missing1_implies_any : forall (state: TwoDiskBaseAPI.State) P,
+      disk1 state ?|= missing ->
+      disk1 state ?|= P.
+  Proof.
+    destruct state; unfold missing; simpl; intuition auto.
+  Qed.
+
+  Hint Resolve missing0_implies_any.
+  Hint Resolve missing1_implies_any.
+
+  Theorem read_int_ok : forall a,
+      proc_ok TDLayer
+        (read a)
+        td.recover
+        (fun d state =>
+           {|
+             pre := disk0 state ?|= eq d /\
+                    disk1 state ?|= eq d;
+             post :=
+               fun state' r =>
+                 diskGet d a ?|= eq r /\
+                 disk0 state' ?|= eq d /\
+                 disk1 state' ?|= eq d;
+             recovered :=
+               fun state' _ =>
+                 disk0 state' ?|= eq d /\
+                 disk1 state' ?|= eq d;
+           |}).
+  Proof.
+    unfold read.
+    step.
+    destruct r; step.
+    destruct r; step.
+  Qed.
+
+  Hint Resolve read_int_ok.
+
+  Theorem write_int_ok : forall a b,
+      proc_ok TDLayer
+        (write a b)
+        td.recover
+        (fun d state =>
+           {|
+             pre :=
+               disk0 state ?|= eq d /\
+               disk1 state ?|= eq d;
+             post :=
+               fun state' r =>
+                 r = tt /\
+                 disk0 state' ?|= eq (diskUpd d a b) /\
+                 disk1 state' ?|= eq (diskUpd d a b);
+             recovered :=
+               fun state' _ =>
+                 (disk0 state' ?|= eq d /\
+                  disk1 state' ?|= eq d) \/
+                 (a < diskSize d /\
+                  disk0 state' ?|= eq (diskUpd d a b) /\
+                  disk1 state' ?|= eq d) \/
+                 (disk0 state' ?|= eq (diskUpd d a b) /\
+                  disk1 state' ?|= eq (diskUpd d a b));
+           |}).
+  Proof.
+    unfold write.
+    step.
+
+    destruct r; step.
+    descend; intuition eauto.
+
+    step.
+    destruct r; (intuition eauto); simplify.
+    destruct (lt_dec a (diskSize a')).
+    eauto.
+    simplify.
+
+    destruct r; step.
+  Qed.
+
+  Hint Resolve write_int_ok.
+
+  Theorem size_int_ok :
+    proc_ok TDLayer
+      (size)
+      td.recover
+      (fun '(d_0, d_1) state =>
+         {|
+           pre :=
+             disk0 state ?|= eq d_0 /\
+             disk1 state ?|= eq d_1 /\
+             diskSize d_0 = diskSize d_1;
+           post :=
+             fun state' r =>
+               r = diskSize d_0 /\
+               r = diskSize d_1 /\
+               disk0 state' ?|= eq d_0 /\
+               disk1 state' ?|= eq d_1;
+           recovered :=
+             fun state' _ =>
+               disk0 state' ?|= eq d_0 /\
+               disk1 state' ?|= eq d_1;
+         |}).
+  Proof.
+    unfold size.
+    step.
+    destruct r; step.
+    destruct r; step.
+  Qed.
+
+  Hint Resolve size_int_ok.
+
+  Definition equal_after a (d_0 d_1: disk) :=
+    diskSize d_0 = diskSize d_1 /\
+    forall a', a <= a' -> diskGet d_0 a' = diskGet d_1 a'.
+
+  Theorem le_eq_or_S_le : forall n m,
+      n <= m ->
+      n = m \/
+      S n <= m /\ n <> m.
+  Proof.
+    intros.
+    omega.
+  Qed.
+
+  Theorem equal_after_diskUpd : forall a d_0 d_1 b,
+      equal_after (S a) d_0 d_1 ->
+      equal_after a (diskUpd d_0 a b) (diskUpd d_1 a b).
+  Proof.
+    unfold equal_after; intuition.
+    autorewrite with upd; eauto.
+    apply le_eq_or_S_le in H; intuition subst.
+    destruct (lt_dec a' (diskSize d_0)); autorewrite with upd.
+    assert (a' < diskSize d_1) by congruence; autorewrite with upd; auto.
+    assert (~a' < diskSize d_1) by congruence; autorewrite with upd; auto.
+    autorewrite with upd; eauto.
+  Qed.
+
+  Hint Resolve equal_after_diskUpd.
+
+  (*
+  Theorem init_at_ok : forall a,
+      proc_ok TDLayer
+        (init_at a)
+        td.recover
+        (fun '(d_0, d_1) state =>
+           {| pre :=
+                disk0 state ?|= eq d_0 /\
+                disk1 state ?|= eq d_1 /\
+                equal_after a d_0 d_1;
+              post :=
+                fun state' _ =>
+                  exists d_0' d_1': disk,
+                    disk0 state' ?|= eq d_0' /\
+                    disk1 state' ?|= eq d_1' /\
+                    equal_after 0 d_0' d_1';
+              recovered :=
+                fun state' _ => True;
+           |}).
+  Proof.
+    induction a; simpl; intros.
+    - step.
+    - step.
+
+      step.
+      destruct r; finish.
+      + step.
+        destruct r; simplify; finish.
+      + step.
+        destruct r; finish.
+  Qed.
+
+  Hint Resolve init_at_ok.
+
+  Theorem sizeInit_ok :
+    proc_ok TDLayer
+      (sizeInit)
+      td.recover
+      (fun '(d_0, d_1) state =>
+         {| pre :=
+              disk0 state ?|= eq d_0 /\
+              disk1 state ?|= eq d_1;
+            post :=
+              fun state' r =>
+                exists d_0' d_1',
+                  disk0 state' ?|= eq d_0' /\
+                  disk1 state' ?|= eq d_1' /\
+                  match r with
+                  | Some sz => diskSize d_0' = sz /\ diskSize d_1' = sz
+                  | None => True
+                  end;
+            recovered :=
+              fun state' _ => True;
+         |}).
+  Proof.
+    unfold sizeInit.
+    step.
+    destruct r.
+    step.
+    - destruct r.
+      + destruct (diskSize d_0 == v).
+        * step.
+        * step.
+      + step.
+    - step.
+      destruct r.
+      + step.
+      + step.
+  Qed.
+
+  Hint Resolve sizeInit_ok.
+   *)
+
+
+  Theorem equal_after_0_to_eq : forall d_0 d_1,
+      equal_after 0 d_0 d_1 ->
+      d_0 = d_1.
+  Proof.
+    unfold equal_after; intuition.
+    eapply disk_ext_eq; intros.
+    eapply H1; omega.
+  Qed.
+
+  Theorem equal_after_size : forall d_0 d_1,
+      diskSize d_0 = diskSize d_1 ->
+      equal_after (diskSize d_0) d_0 d_1.
+  Proof.
+    unfold equal_after; intuition.
+    assert (~a' < diskSize d_0) by omega.
+    assert (~a' < diskSize d_1) by congruence.
+    autorewrite with upd; eauto.
+  Qed.
+
+  Hint Resolve equal_after_size.
+  Hint Resolve equal_after_0_to_eq.
+
+  (*
+  Theorem init'_ok :
+    proc_ok TDLayer
+      (init')
+      td.recover
+      (fun '(d_0, d_1) state =>
+         {| pre :=
+              disk0 state ?|= eq d_0 /\
+              disk1 state ?|= eq d_1;
+            post :=
+              fun r state' =>
+                match r with
+                | Initialized =>
+                  exists d_0' d_1',
+                  disk0 state' ?|= eq d_0' /\
+                  disk1 state' ?|= eq d_1' /\
+                  d_0' = d_1'
+                | InitFailed =>
+                  True
+                end;
+            recovered :=
+              fun _ state' => True;
+         |}).
+  Proof.
+    unfold init.
+    step.
+    descend; intuition eauto.
+    destruct r; step.
+    step.
+  Qed.
+
+  Hint Resolve init'_ok.
+   *)
+
+  (**
+   * Recovery implementation.
+   *
+   * General structure for recovery: essentially, it consists of
+   * a loop around [fixup] that terminates after either fixing an out-of-sync
+   * disk block or when a disk has failed.
+  *)
+
+  (* [fixup] returns a [RecStatus] to implement early termination in [recovery_at]. *)
+  Inductive RecStatus :=
+  (* continue working, nothing interesting has happened *)
+  | Continue
+  (* some address has been repaired (or the recovery has exhausted the
+     addresses) - only one address can be out of sync and thus only it must be
+     recovered. *)
+  (* OR, one of the disks has failed, so don't bother continuing recovery since
+     the invariant is now trivially satisfied *)
+  | RepairDoneOrFailed.
+
+  Definition fixup (a:addr) : proc Op RecStatus :=
+    mv0 <- td.read d0 a;
+    match mv0 with
+    | Working v =>
+      mv2 <- td.read d1 a;
+      match mv2 with
+      | Working v' =>
+        if v == v' then
+          Ret Continue
+        else
+          mu <- td.write d1 a v;
+          Ret RepairDoneOrFailed
+      | Failed => Ret RepairDoneOrFailed
+      end
+    | Failed => Ret RepairDoneOrFailed
+    end.
+
+  (* recursively performs recovery at [a-1], [a-2], down to 0 *)
+  Fixpoint recover_at (a:addr) : proc Op unit :=
+    match a with
+    | 0 => Ret tt
+    | S n =>
+      s <- fixup n;
+      match s with
+      | Continue => recover_at n
+      | RepairDoneOrFailed => Ret tt
+      end
+    end.
+
+  Definition Recover : proc Op unit :=
+    sz <- size;
+    _ <- recover_at sz;
+    Ret tt.
+
+
+  (**
+   * Theorems and recovery proofs.
+   *)
+
+  Theorem if_lt_dec : forall A n m (a a':A),
+      n < m ->
+      (if lt_dec n m then a else a') = a.
+  Proof.
+    intros.
+    destruct (lt_dec n m); auto.
+    contradiction.
+  Qed.
+
+  Theorem disks_eq_inbounds : forall (d: disk) a v v',
+      a < diskSize d ->
+      diskGet d a ?|= eq v ->
+      diskGet d a ?|= eq v' ->
+      v = v'.
+  Proof.
+    intros.
+    case_eq (diskGet d a); intros.
+    - rewrite H2 in *. simpl in *. congruence.
+    - exfalso.
+      eapply disk_inbounds_not_none; eauto.
+  Qed.
+
+  (* To make these specifications precise while also covering both the already
+   * synced and diverged disks cases, we keep track of which input state we're
+   * in from the input and use it to give an exact postcondition. *)
+  Inductive DiskStatus :=
+  | FullySynced
+  | OutOfSync (a:addr) (b:block).
+
+  Theorem diskUpd_maybe_same : forall (d:disk) a b,
+      diskGet d a ?|= eq b ->
+      diskUpd d a b = d.
+  Proof.
+    intros.
+    destruct (diskGet d a) eqn:?; simpl in *; subst;
+      autorewrite with upd;
+      auto.
+  Qed.
+
+  Hint Rewrite diskUpd_maybe_same using (solve [ auto ]) : upd.
+  Hint Resolve PeanoNat.Nat.lt_neq.
+  Hint Resolve disks_eq_inbounds.
+
+  (* we will show that fixup does nothing once the disks are the same *)
+  Theorem fixup_equal_ok : forall a,
+      proc_ok TDLayer
+        (fixup a)
+        td.recover
+        (fun d state =>
+           {|
+             pre :=
+               (* for simplicity we only consider in-bounds addresses, though
+                  if a is out-of-bounds fixup just might uselessly write to
+                  disk and not do anything *)
+               a < diskSize d /\
+               disk0 state ?|= eq d /\
+               disk1 state ?|= eq d;
+             post :=
+               fun state' r =>
+                 disk0 state' ?|= eq d /\
+                 disk1 state' ?|= eq d;
+             recovered :=
+               fun state' _ =>
+                 disk0 state' ?|= eq d /\
+                 disk1 state' ?|= eq d;
+           |}).
+  Proof.
+    unfold fixup.
+    step.
+
+    destruct r; step.
+
+    destruct r; try step.
+    destruct (v == v0); subst; try step.
+
+    Unshelve.
+    auto.
+    exact (fun _ => True).
+  Qed.
+
+  Theorem fixup_correct_addr_ok : forall a,
+      proc_ok TDLayer
+        (fixup a)
+        td.recover
+        (fun '(d, b) state =>
+           {|
+             pre :=
+               a < diskSize d /\
+               disk0 state ?|= eq (diskUpd d a b) /\
+               disk1 state ?|= eq d;
+             post :=
+               fun state' r =>
+                 match r with
+                 | Continue =>
+                   (* could happen if b already happened to be value *)
+                   disk0 state' ?|= eq (diskUpd d a b) /\
+                   disk1 state' ?|= eq (diskUpd d a b)
+                 | RepairDoneOrFailed =>
+                   (disk0 state' ?|= eq (diskUpd d a b) /\
+                    disk1 state' ?|= eq (diskUpd d a b)) \/
+                   (disk0 state' ?|= eq d /\
+                    disk1 state' ?|= eq d)
+                 end;
+             recovered :=
+               fun state' _ =>
+                 (disk0 state' ?|= eq (diskUpd d a b) /\
+                  disk1 state' ?|= eq (diskUpd d a b)) \/
+                 (disk0 state' ?|= eq (diskUpd d a b) /\
+                  disk1 state' ?|= eq d) \/
+                 (disk0 state' ?|= eq d /\
+                  disk1 state' ?|= eq d);
+           |}).
+  Proof.
+    unfold fixup; intros.
+    step.
+
+    destruct r; try step.
+
+    destruct r; try step.
+    destruct (b == v); subst; try step.
+
+    step.
+    destruct r; simplify; finish.
+  Qed.
+
+  Theorem fixup_wrong_addr_ok : forall a,
+      proc_ok TDLayer
+        (fixup a)
+        td.recover
+        (fun '(d, b, a') state =>
+           {|
+             pre :=
+               a < diskSize d /\
+               (* recovery, working from end of disk, has not yet reached the
+                  correct address *)
+               a' < a /\
+               disk0 state ?|= eq (diskUpd d a' b) /\
+               disk1 state ?|= eq d;
+             post :=
+               fun state' r =>
+                 match r with
+                 | Continue =>
+                   disk0 state' ?|= eq (diskUpd d a' b) /\
+                   disk1 state' ?|= eq d
+                 | RepairDoneOrFailed =>
+                   (disk0 state' ?|= eq d /\
+                    disk1 state' ?|= eq d) \/
+                   (disk0 state' ?|= eq (diskUpd d a' b) /\
+                    disk1 state' ?|= eq (diskUpd d a' b))
+                 end;
+             recovered :=
+               fun state' _ =>
+                 (disk0 state' ?|= eq (diskUpd d a' b) /\
+                  disk1 state' ?|= eq d) \/
+                 (disk0 state' ?|= eq d /\
+                  disk1 state' ?|= eq d);
+           |}).
+  Proof.
+    unfold fixup; intros.
+    step.
+
+    destruct r; try step.
+    destruct r; try step.
+
+    destruct (v == v0); subst.
+    step.
+
+    step.
+    Unshelve.
+    auto.
+    exact (fun _ => True).
+  Qed.
+
+  Ltac spec_case pf :=
+    eapply spec_impl_relations; [ unfold spec_impl | solve [ apply pf ] ].
+
+
+  Theorem fixup_ok : forall a,
+      proc_ok TDLayer
+        (fixup a)
+        td.recover
+        (fun '(d, s) state =>
+           {|
+             pre :=
+               a < diskSize d /\
+               match s with
+               | FullySynced => disk0 state ?|= eq d /\
+                               disk1 state ?|= eq d
+               | OutOfSync a' b => a' <= a /\
+                                  disk0 state ?|= eq (diskUpd d a' b) /\
+                                  disk1 state ?|= eq d
+               end;
+             post :=
+               fun state' r =>
+                 match s with
+                 | FullySynced => disk0 state' ?|= eq d /\
+                                 disk1 state' ?|= eq d
+                 | OutOfSync a' b =>
+                   match r with
+                   | Continue =>
+                     (a' < a /\
+                      disk0 state' ?|= eq (diskUpd d a' b) /\
+                      disk1 state' ?|= eq d) \/
+                     (disk0 state' ?|= eq (diskUpd d a' b) /\
+                      disk1 state' ?|= eq (diskUpd d a' b))
+                   | RepairDoneOrFailed =>
+                     (disk0 state' ?|= eq d /\
+                      disk1 state' ?|= eq d) \/
+                     (disk0 state' ?|= eq (diskUpd d a' b) /\
+                      disk1 state' ?|= eq (diskUpd d a' b))
+                   end
+                 end;
+             recovered :=
+               fun state' _ =>
+                 match s with
+                 | FullySynced => disk0 state' ?|= eq d /\
+                                 disk1 state' ?|= eq d
+                 | OutOfSync a' b =>
+                   (disk0 state' ?|= eq (diskUpd d a' b) /\
+                    disk1 state' ?|= eq (diskUpd d a' b)) \/
+                   (disk0 state' ?|= eq (diskUpd d a' b) /\
+                    disk1 state' ?|= eq d) \/
+                   (disk0 state' ?|= eq d /\
+                    disk1 state' ?|= eq d)
+                 end;
+           |}).
+  Proof.
+    spec_intros; simplify.
+    destruct s; intuition eauto.
+    - spec_case fixup_equal_ok; simplify; finish.
+    - apply PeanoNat.Nat.lt_eq_cases in H1; intuition.
+      + spec_case fixup_wrong_addr_ok; simplify; finish.
+        repeat apply exists_tuple2; simpl.
+        exists d, b, a0.
+        simplify; finish.
+
+        destruct v; finish.
+      + spec_case fixup_correct_addr_ok; simplify; finish.
+        exists d, b.
+        simplify; finish.
+
+        destruct v; finish.
+  Qed.
+
+  Hint Resolve fixup_ok.
+
+  (* Hint Resolve Lt.lt_n_Sm_le. *)
+
+  Theorem recover_at_ok : forall a,
+      proc_ok TDLayer
+        (recover_at a)
+        td.recover
+        (fun '(d, s) state =>
+           {|
+             pre :=
+               a <= diskSize d /\
+               match s with
+               | FullySynced => disk0 state ?|= eq d /\
+                               disk1 state ?|= eq d
+               | OutOfSync a' b => a' < a /\
+                                  disk0 state ?|= eq (diskUpd d a' b) /\
+                                  disk1 state ?|= eq d
+               end;
+             post :=
+               fun state' r =>
+                 match s with
+                 | FullySynced =>
+                   disk0 state' ?|= eq d /\
+                   disk1 state' ?|= eq d
+                 | OutOfSync a' b =>
+                   (disk0 state' ?|= eq d /\
+                    disk1 state' ?|= eq d) \/
+                   (disk0 state' ?|= eq (diskUpd d a' b) /\
+                    disk1 state' ?|= eq (diskUpd d a' b))
+                 end;
+             recovered :=
+               fun state' _ =>
+                 match s with
+                 | FullySynced => disk0 state' ?|= eq d /\
+                                 disk1 state' ?|= eq d
+                 | OutOfSync a' b =>
+                   (disk0 state' ?|= eq d /\
+                    disk1 state' ?|= eq d) \/
+                   (disk0 state' ?|= eq (diskUpd d a' b) /\
+                    disk1 state' ?|= eq d) \/
+                   (disk0 state' ?|= eq (diskUpd d a' b) /\
+                    disk1 state' ?|= eq (diskUpd d a' b))
+                 end;
+           |}).
+  Proof.
+    induction a; simpl; intros.
+    - step.
+      destruct s; simplify.
+    - step.
+      destruct s; simplify.
+      exists d, FullySynced; simplify; finish.
+      destruct r; step.
+
+      exists d, FullySynced; simplify; finish.
+      omega.
+      exists d, (OutOfSync a0 b); simplify; finish.
+      intuition eauto.
+      omega.
+
+      destruct r; step.
+      intuition.
+      exists d, (OutOfSync a0 b); simplify; finish.
+      omega.
+      exists (diskUpd d a0 b), FullySynced; simplify; finish.
+      omega.
+  Qed.
+
+  Hint Resolve recover_at_ok.
+
+  Definition Recover_spec : Specification _ unit unit TwoDiskBaseAPI.State :=
+    fun '(d, s) state =>
+      {|
+        pre :=
+          match s with
+          | FullySynced => disk0 state ?|= eq d /\
+                          disk1 state ?|= eq d
+          | OutOfSync a b => a < diskSize d /\
+                            disk0 state ?|= eq (diskUpd d a b) /\
+                            disk1 state ?|= eq d
+          end;
+        post :=
+          fun state' (_:unit) =>
+            match s with
+            | FullySynced => disk0 state' ?|= eq d /\
+                            disk1 state' ?|= eq d
+            | OutOfSync a b =>
+              (disk0 state' ?|= eq d /\
+               disk1 state' ?|= eq d) \/
+              (disk0 state' ?|= eq (diskUpd d a b) /\
+               disk1 state' ?|= eq (diskUpd d a b))
+            end;
+        recovered :=
+          fun state' (_:unit) =>
+            match s with
+            | FullySynced => disk0 state' ?|= eq d /\
+                            disk1 state' ?|= eq d
+            | OutOfSync a b =>
+              (disk0 state' ?|= eq d /\
+               disk1 state' ?|= eq d) \/
+              (disk0 state' ?|= eq (diskUpd d a b) /\
+               disk1 state' ?|= eq d) \/
+              (disk0 state' ?|= eq (diskUpd d a b) /\
+               disk1 state' ?|= eq (diskUpd d a b))
+            end;
+      |}.
+
+  Theorem Recover_rok :
+    proc_ok TDLayer
+      (Recover)
+      td.recover
+      Recover_spec.
+  Proof.
+    unfold Recover, Recover_spec; intros.
+    spec_intros; simplify.
+    destruct s; simplify.
+    + step.
+      step.
+      exists d, FullySynced; simplify; finish.
+
+      step.
+
+    + step.
+      intuition eauto.
+      simplify.
+      step.
+
+      exists d, (OutOfSync a b); simplify; finish.
+      step.
+  Qed.
+
+  Theorem Recover_spec_idempotent :
+    idempotent Recover_spec.
+  Proof.
+    unfold idempotent; intuition; simplify.
+    rename a0 into d.
+    destruct b; intuition eauto.
+    - exists d, FullySynced; finish.
+    - exists d, FullySynced; finish.
+    - exists d, (OutOfSync a b); finish.
+    - exists (diskUpd d a b), FullySynced; finish.
+  Qed.
+
+  (* TODO: not sure this is the right level to prove this looping lemma *)
+  (* This proof combines your proof that recovery is correct and that its
+  specification is idempotent to show recovery is correct even if re-run on
+  every crash. *)
+  (*
+  Theorem Recover_ok :
+    proc_loopspec
+      Recover_spec
+      (Recover)
+      td.recover
+      td.abstr.
+  Proof.
+    eapply idempotent_loopspec; simpl.
+    - apply Recover_rok.
+    - apply Recover_spec_idempotent.
+  Qed.
+   *)
+
+  (*
+  Hint Resolve Recover_ok.
+   *)
+
+  Definition recover: proc Op unit :=
+    _ <- td.recover;
+    Recover.
+
+  (* As the final step in giving the correctness of the replicated disk
+  operations, we prove recovery specs that include the replicated disk Recover
+  function. *)
+
+  Definition rd_abstraction (d:OneDiskAPI.State) (state: TwoDiskBaseAPI.State)  (_ :unit) : Prop :=
+    disk0 state ?|= eq d /\
+    disk1 state ?|= eq d.
+
+  Definition Impl_TD_OD: LayerImpl Op OneDiskOp :=
+    {| compile_op := fun (T : Type) (op : OneDiskOp T) =>
+                       match op in (OneDiskOp T0) return (proc Op T0) with
+                       | op_read a => read a
+                       | op_write a b => write a b
+                       | op_size => size
+                       end;
+       Layer.recover := recover |}.
+
+  Import Helpers.RelationAlgebra.
+  Import RelationNotations.
+
+  (*
+  Lemma compile_refine_TD_OD:
+    compile_op_refines_step TDLayer ODLayer Impl_TD_OD rd_abstraction.
+  Proof.
+    unfold compile_op_refines_step.
+    intros T op. destruct op.
+    - unfold crash_refines, refines. split.
+      * SearchAbout and_then.
+        rewrite <-
+        rewrite  apply and_then_monotonic_r.
+
+
+  Lemma Refinement_TD_OD: LayerRefinement TDLayer ODLayer.
+  Proof.
+    unshelve (econstructor).
+    - apply Impl_TD_OD. 
+    - exact rd_abstraction.
+      Show Proof.
+      simpl. Check rd_abstraction. Che Print relation. apply @rd_abstraction.
+    refine {| impl := Impl_TD_OD;
+              absr := rd_abstraction
+           |}.
+    - 
+    econstructor.
+    split.
+
+  Definition abstr : Abstraction OneDiskAPI.State :=
+    abstraction_compose td.abstr {| abstraction := rd_abstraction; |}.
+
+  Theorem init_ok : init_abstraction init recover abstr inited_any.
+  Proof.
+    intros.
+    eapply then_init_compose; eauto.
+    eapply proc_spec_weaken; eauto.
+    unfold spec_impl; intros.
+    destruct state; simpl in *.
+
+    - exists (d_0, d_1); simpl; intuition eauto.
+      unfold rd_abstraction.
+      destruct v; repeat deex; eauto.
+    - exists (d_0, d_0); simpl; intuition eauto.
+      unfold rd_abstraction.
+      destruct v; repeat deex; eauto.
+    - exists (d_1, d_1); simpl; intuition eauto.
+      unfold rd_abstraction.
+      destruct v; repeat deex; eauto.
+  Qed.
+
+
+  Theorem read_ok : forall a, proc_spec (read_spec a) (read a) recover abstr.
+  Proof.
+    intros.
+    apply spec_abstraction_compose; simpl.
+    eapply compose_recovery; eauto; simplify.
+    unfold rd_abstraction in *; descend; intuition eauto.
+    exists (state2, FullySynced); simplify; finish.
+  Qed.
+
+  Theorem write_ok : forall a v, proc_spec (write_spec a v) (write a v) recover abstr.
+  Proof.
+    intros.
+    apply spec_abstraction_compose; simpl.
+    eapply compose_recovery; eauto; simplify.
+    rename state2 into d.
+    unfold rd_abstraction in *; descend; intuition eauto.
+    - exists (d, FullySynced); simplify; intuition eauto.
+    - exists (d, OutOfSync a v); simplify; intuition eauto.
+    - exists (diskUpd d a v, FullySynced); simplify; intuition eauto.
+  Qed.
+
+  Theorem size_ok : proc_spec size_spec size recover abstr.
+  Proof.
+    intros.
+    apply spec_abstraction_compose; simpl.
+    (* simplify is a bit too aggressive about existential variables here, so we
+    provide some manual simplification here *)
+    eapply compose_recovery; eauto.
+    intros; apply exists_tuple2.
+    destruct a; simpl in *.
+    rename s into d.
+    unfold rd_abstraction in *; simplify.
+    exists d, d; intuition eauto.
+    simplify.
+    exists d, FullySynced; simplify; finish.
+  Qed.
+
+  (* This theorem shows that Ret does not modify the abstract state exposed by
+  the replicated disk; the interesting part is that if recovery runs, then the
+  only effect should be the wipe relation (the trivial relation [no_wipe] in
+  this case) *)
+  Theorem recover_noop : rec_noop recover abstr no_wipe.
+  Proof.
+    eapply rec_noop_compose; eauto; simpl.
+    autounfold; unfold rd_abstraction, Recover_spec; simplify.
+    exists state0', FullySynced; intuition eauto.
+  Qed.
+   *)
+
+End ReplicatedDisk.
